\subsection{Mortality-free annuities}

Constant payment discrete annuities:
\begin{itemize}
\item Annuity due
\begin{equation*}
\ax**{\angln} = 1 + v + v^2 + \cdots + v^{n - 1} = \frac{1 - v^n}{1 - v} = \frac{1 - v^n}{d}.
\end{equation*}
\item Annuity immediate
\begin{equation*}
\ax{\angln} = v\ax**{\angln} = \frac{1 - v^n}{i}
\end{equation*}
\item Accumulated value of annuity due
\begin{equation*}
\sx**{\angln} = (1 + i)^n\ax**{\angln} = \frac{(1 + i)^n - 1}{d}
\end{equation*}
\item Accumulated value of annuity immediate
\begin{equation*}
\sx{\angln} = v\sx**{\angln} = \frac{(1 + i)^n - 1}{i}
\end{equation*}
\end{itemize}

\newpage
Non-constant payment discrete annuities (due versions):
\begin{itemize}
\item Increasing annuity
\begin{equation*}
\begin{split}
\Ia**_{\angln} &= 1 + 2v + 3v^2 + \cdots + nv^{n - 1} = \frac{\partial}{\partial v}\left(\frac{1 - v^{n + 1}}{1 - v}\right) \\
&= \frac{(1 - v)(-(n + 1)v^n) - (1 - v^{n + 1})(-1)}{(1 - v)^2} = \frac{nv^{n + 1} - (n + 1)v^n + 1}{(1 - v)^2} \\
&= \frac{nv^n(v - 1) + 1 - v^n}{d^2} = \frac{\ax**{\angln} - nv^n}{d}
\end{split}
\end{equation*}
\item Decreasing annuity
\begin{equation*}
\begin{split}
\Da**_{\angln} &= n + (n - 1)v + (n - 2)v^2 + \cdots + v^{n - 1} = (n + 1)\ax**{\angln} - \Ia**_{\angln} \\
&= \frac{d(n + 1)\ax**{\angln} - (\ax**{\angln} - nv^n)}{d} = \frac{(n + 1)(1 - v^n) - \ax**{\angln} + nv^n}{d} \\
&= \frac{n + 1 - \ax**{\angln} - v^n}{d} = \frac{n - \ax{\angln}}{d}.
\end{split}
\end{equation*}
\end{itemize}

Perpetuities (due versions):
\begin{itemize}
\item Constant
\begin{equation*}
\ax**{\angl{\infty}} = \lim_{n\to\infty}\ax**{\angln} = \frac{1}{d}
\end{equation*}
\item Increasing
\begin{equation*}
\Ia**_{\angl{\infty}} = \lim_{n\to\infty}\Ia**_{\angln} = \frac{1}{d^2}
\end{equation*}
\end{itemize}

Payments split $m$th-ly:
\begin{itemize}
\item Constant annuity due
\begin{equation*}
\ax**{\angln}[(m)] = \frac{1}{m}(1 + v^{1/m} + \cdots + v^{n - 1/m}) = \frac{1}{m}\frac{1 - v^n}{1 - v^{1/m}} = \frac{1 - v^n}{d^{(m)}}
\end{equation*}
\item Constant annuity immediate
\begin{equation*}
\ax{\angln}[(m)] = v^{1/m}\ax**{\angln}[(m)] = \frac{1 - v^n}{i^{(m)}}
\end{equation*}
\item Increasing annuity due
\begin{equation*}
\begin{split}
\Ia**_{\angln}^{(m)} &= \frac{1}{m} + \frac{2}{m}v^{1/m} + \cdots + nv^{n - 1/m} \\
&= \frac{mnv^n(v^{1/m} - 1) + 1 - v^n}{m(1 - v^{1/m})^2} = \frac{\ax**{\angln}[(m)] - nv^n}{d^{(m)}}
\end{split}
\end{equation*}
\end{itemize}

\newpage
Continuous annuities:
\begin{itemize}
\item Constant
\begin{equation*}
\ax*{\angln} = \lim_{m\to\infty} \ax**{\angln}[(m)] = \frac{1 - v^n}{\delta} = \int_0^n v^t\,dt
\end{equation*}
\item Increasing 
\begin{equation*}
\Ia*_{\angln} = \lim_{m\to\infty} \Ia**_{\angln}^{(m)} = \frac{\ax*{\angln} - nv^n}{\delta} = \int_0^n tv^t\,dt
\end{equation*}
\end{itemize}