\subsection{Discrete life insurance}

Assumptions and notation
\begin{itemize}
\item Benefit $b_{K + 1}$ paid at the end of the year of death
\item Constant interest rate
\item Payout random variable $Z$
\end{itemize}

Whole life insurance
\begin{itemize}
\item $Z = b_{K + 1}v^{K + 1}$
\item Expected value $\mathbb{E}[Z] = \sum_{k = 0}^{\infty} b_{k + 1}v^{k + 1}\qx[k|]{x}$
\item Second moment $\mathbb{E}[Z^2] = \sum_{k = 0}^{\infty} b_{k + 1}^2v^{2(k + 1)}\qx[k|]{x}$ equivalent to expected value of $Z$ for benefit $b_{k + 1}^{*} = b_{k + 1}^2$ and interest $i^{*} = (1 + i)^2 - 1$, i.e. $v^{*} = v^2$ or $\delta^{*} = 2\delta$
\item If $b_{k + 1} = 1$ throughout, define $\Ax{x} = \mathbb{E}[Z]$ and $\Ax[][2]{x} = \mathbb{E}[Z^2]$
\item DML mortality law
\begin{align*}
\Ax{x} &= \sum_{k = 0}^{\omega - x - 1}\frac{v^{k + 1}}{\omega - x} = \frac{\ax{\angl{\omega - x}}}{\omega - x} \\
\Ax[][2]{x} &= \sum_{k = 0}^{\omega - x - 1}\frac{v^{2(k + 1)}}{\omega - x} = \frac{\ax{\angl{\omega - x}i^{*}}}{\omega - x}
\end{align*}
\item CFM mortality law
\begin{align*}
\Ax{x} &= \sum_{k = 0}^{\infty} v^{k + 1}e^{-\mu k}(1 - e^{-\mu}) = v(1 - e^{-\mu})\sum_{k = 0}^{\infty} (ve^{-\mu})^k \\
&= e^{-\delta}(1 - e^{-\mu})\cdot\frac{1}{1 - e^{-(\delta + \mu)}} = \frac{e^{-\delta}(1 - e^{-\mu})}{1 - e^{-(\delta + \mu)}} \\
\Ax[][2]{x} &= \sum_{k = 0}^{\infty} v^{2(k + 1)}e^{-\mu k}(1 - e^{-\mu}) = \frac{e^{-\delta^{*}}(1 - e^{-\mu})}{1 - e^{-(\delta^{*} + \mu)}}
\end{align*}
\end{itemize}

$n$-year term insurance
\begin{itemize}
\item $Z = \begin{cases} b_{K + 1}v^{K + 1} & K < n \\ 0 & K\geq n \end{cases}$
\item Expected value $\mathbb{E}[Z] = \sum_{k = 0}^{n - 1} b_{k + 1}v^{k + 1}\qx[k|]{x}$
\item Second moment $\mathbb{E}[Z^2] = \sum_{k = 0}^{n - 1} b_{k + 1}^2v^{2(k + 1)}\qx[k|]{x}$
\item If $b_{k + 1} = 1$ for $k < n$, define $\Ax{\term{x}{n}} = \mathbb{E}[Z]$
\item DML mortality law: if $n' = \min\{n, \omega - x\}$, then
\begin{align*}
\Ax{\term{x}{n}} &= \frac{\ax{\angl{n'}}}{\omega - x} \\
\Ax[][2]{\term{x}{n}} &= \frac{\ax{\angl{n'}i^{*}}}{\omega - x}
\end{align*}
\item CFM mortality law
\begin{align*}
\Ax{\term{x}{n}} &= v(1 - e^{-\mu})\sum_{k = 0}^{n - 1} (ve^{-\mu})^k = e^{-\delta}(1 - e^{-\mu})\cdot\frac{1 - e^{-n(\delta + \mu)}}{1 - e^{-(\delta + \mu)}} \\
\Ax[][2]{\term{x}{n}} &= e^{-\delta^{*}}(1 - e^{-\mu})\cdot\frac{1 - e^{-n(\delta^{*} + \mu)}}{1 - e^{-(\delta^{*} + \mu)}}
\end{align*}
\end{itemize}

$n$-year pure endowment
\begin{itemize}
\item $Z = 0$ if $K < n$ and $Z = bv^n$ if $K\geq n$, where $b$ is benefit paid out for surviving
\item Expected value $\mathbb{E}[Z] = bv^n\mathbb{P}[K\geq n] = bv^n\px[n]{x}$
\item Second moment $\mathbb{E}[Z^2] = b^2v^{2n}\px[n]{x}$
\item If $b = 1$, define $\Ax{\pureendow{x}{n}} = \Ex[n]{x} = \mathbb{E}[Z] = v^n\px[n]{x}$
\end{itemize}

$n$-year (endowment) insurance
\begin{itemize}
\item $Z = Z_{n\text{-year terminsurance}} + Z_{n\text{-year pure endowment}} = \begin{cases} b_{K + 1}v^{K + 1} & K < n \\ bv^n & K\geq n \end{cases}$
\item If $b_{k + 1} = 1$ for $k < n$ and $b = 1$, define $\Ax{\endow{x}{n}} = \mathbb{E}[Z] = \Ax{\term{x}{n}} + \Ex[n]{x}$
\end{itemize}

Recurrences
\begin{itemize}
\item $\Ax{x} = \Ax{\term{x}{n}} + \Ex[n]{x}\cdot\Ax{x + n}$
\item $\Ax{\term{x}{n}} = \Ax{\term{x}{k}} + \Ex[k]{x}\cdot\Ax{\term{x + k}{n - k}}$ for $0\leq k\leq n$
\end{itemize}